refine composition of multi transition relations

src/tools/parallelcomposition/interleavingScript.sml
@@ -7,18 +7,40 @@ open pairTheory wordsTheory set_sepTheory;
 open quantHeuristicsTheory;
 open propertyTheory;
 val _ = new_theory "interleaving";
-    
-(* Trace *)
-val _ = Parse.type_abbrev("trc", ``:'event list``);  
 
+
+Inductive MTrn1:
+[~nil:]
+  (MTrn1 ((v:'symb),(p:'pred1),(s:'state1)) ([]:('event1+'eventS) list) (v,p,s)) /\
+[~snoc:]
+  ((( MTrn1 (v,p,s) t (v',p',s')) /\ ( MTrn1 (v',p',s') [e] (v'',p'',s''))) ==> ( MTrn1 (v,p,s) (e::t) (v'',p'',s'')))
+End
+
+Inductive MTrn2:
+[~nil:]
+  (MTrn2 ((v:'symb),(p:'pred2),(s:'state2)) ([]:('event2+'eventS) list) (v,p,s)) /\
+[~snoc:]
+  ((( MTrn2 (v,p,s) t (v',p',s')) /\ ( MTrn2 (v',p',s') [e] (v'',p'',s''))) ==> ( MTrn2 (v,p,s) (e::t) (v'',p'',s'')))
+End        
+(*    
+Inductive comptrace:
+[~nil:]
+  (comptrace (MTrn:( (('event1+'evenS)+('event2+'eventS)), ('pred1+'pred2), 'state1#'state2 , 'symb ) mtrel) (v,p,s1,s2) [] (v,p,s1,s2)) /\
+[~snoc:]
+  (((comptrace MTrn (v,p,s1,s2) t (v',p',s1',s2')) /\ (comptrace MTrn (v',p',s1',s2') [e] (v'',p'',s1'',s2''))) ==> (comptrace MTrn (v,p,s1,s2) (e::t) (v'',p'',s1'',s2'')))
+End
+*)
+                    
 (* Binary interleaving of traces *)
 Inductive binterl:
 [~nil:]
   (binterl [] [] []) /\
 [~left:]
-  (((binterl t1 t2 t) /\ (t1' = (e1::t1)) /\ (t' = ((INL e1)::t))) ==> (binterl t1' t2 t')) /\
+  (((binterl (t1:('event1 + 'eventS) list) (t2:('event2 + 'eventS) list) t) /\ (t1' = ((INL e1)::t1)) /\ (t' = ((INL (INL e1))::t))) ==> (binterl t1' t2 t')) /\
 [~right:]                                                                        
-  (((binterl t1 t2 t) /\ (t2' = (e2::t2)) /\ (t' = ((INR e2)::t))) ==> (binterl t1 t2' t'))
+  (((binterl (t1:('event1 + 'eventS) list) (t2:('event2 + 'eventS) list) t) /\ (t2' = ((INL e2)::t2)) /\ (t' = ((INR (INL e2))::t))) ==> (binterl t1 t2' t')) /\
+[~sync:]                                                                        
+  (((binterl (t1:('event1 + 'eventS) list) (t2:('event2 + 'eventS) list) t) /\ (t1' = ((INR e)::t1)) /\ (t2' = ((INR e)::t2)) /\ (t' = ((INR (INR e))::t))) ==> (binterl t1' t2' t'))
 End
 
 (*
@@ -31,7 +53,7 @@ Definition binterl:
                    )
    
 End
-   *)
+*)   
 
 Definition binterleave_ts:
   binterleave_ts ts1 ts2 = {t| ∃t1 t2. (t1 ∈ ts1) ∧ (t2 ∈ ts2) ∧ (binterl t1 t2 t)}
@@ -39,9 +61,9 @@ End
 
 val binterleave_trace_decomp_thm = store_thm(
   "binterleave_trace_decomp", ``
-∀Sym P S1 S2 Sym' P' S1' S2' (MTrn1:('event1 + 'eventS, 'pred1, 'state1, 'symb) mtrel) (MTrn2:('event2 + 'eventS, 'pred2, 'state2, 'symb) mtrel) CMTrn CDed Ded1 Ded2 t. 
+∀t Sym P S1 S2 Sym' P' S1' S2' (MTrn1:('event1 + 'eventS, 'pred1, 'state1, 'symb) mtrel) (MTrn2:('event2 + 'eventS, 'pred2, 'state2, 'symb) mtrel) Ded1 Ded2. 
 ((FST ((MTrn1,Ded1) || (MTrn2,Ded2))) (Sym,P,S1,S2) t (Sym',P',S1',S2'))
-  ⇔
+⇔
     (∃t1 t2. (MTrn1 (Sym,(IMAGE OUTL P),S1) t1 (Sym',(IMAGE OUTL P'),S1')) ∧ (MTrn2 (Sym,(IMAGE OUTR P),S2) t2 (Sym',(IMAGE OUTR P'),S2')) ∧ (binterl t1 t2 t))``,
 REPEAT GEN_TAC>> EQ_TAC>> rewrite_tac[composeMultiOperation_def]>> rpt strip_tac>>
 cheat);
@@ -49,12 +71,22 @@ cheat);
 val binterleave_composition_thm = store_thm(
   "binterleave_composition_thm",
   ``∀Ded1 Ded2 (MTrn1:('event1 + 'eventS, 'pred1, 'state1, 'symb) mtrel) (MTrn2:('event2 + 'eventS, 'pred2, 'state2, 'symb) mtrel).
-               (binterleave_ts (traces (MTrn1,Ded1)) (traces (MTrn2,Ded2))) = (comptraces ((MTrn1,Ded1) || (MTrn2,Ded2)))
+         (binterleave_ts (traces (MTrn1,Ded1)) (traces (MTrn2,Ded2))) = (comptraces ((MTrn1,Ded1) || (MTrn2,Ded2)))      
 ``,
 REPEAT GEN_TAC>> rewrite_tac[binterleave_ts,composeMultiOperation_def,comptraces_def,traces_def]>>                           FULL_SIMP_TAC (list_ss++pred_setSimps.PRED_SET_ss++boolSimps.LIFT_COND_ss++boolSimps.EQUIV_EXTRACT_ss) [EXTENSION]  >>       gen_tac >> eq_tac >> cheat
                                           
-  );  
+  );
 (*
+val binterleave_composition_one_thm = store_thm(
+  "binterleave_composition_one_thm",
+  ``∀Ded1 Ded2 t1 t2 t Sym P S1 S2 Sym' P' S1' S2' (MTrn1:('event1 + 'eventS, 'pred1, 'state1, 'symb) mtrel) (MTrn2:('event2 + 'eventS, 'pred2, 'state2, 'symb) mtrel).
+          ((trace MTrn1 (Sym,(IMAGE OUTL P),S1) t1 (Sym',(IMAGE OUTL P'),S1')) ∧ (trace MTrn2 (Sym,(IMAGE OUTR P),S2) t2 (Sym',(IMAGE OUTR P'),S2')) ∧ (comptrace (FST ((MTrn1,Ded1) || (MTrn2,Ded2))) (Sym,P,S1,S2) t (Sym',P',S1',S2'))) ⇔ binterl t1 t2 t``,
+                                                                                                                          REPEAT GEN_TAC>> EQ_TAC
+     rewrite_tac[composeMultiOperation_def]>> cheat
+                                          
+  );  
+  
+
 ∀Ded1 Ded2 (MTrn1:('event1 + 'eventS, 'pred1, 'state1, 'symb) mtrel) (MTrn2:('event2 + 'eventS, 'pred2, 'state2, 'symb) mtrel).
                  (binterleave_ts (traces (MTrn1,Ded1)) (traces (MTrn2,Ded2))) = (comptraces ((MTrn1,Ded1) || (MTrn2,Ded2)))
 REPEAT GEN_TAC>>
@@ -73,15 +105,15 @@ Induct_on `x`
 asm_rewrite_tac[composeMuRe_def]
 
 METIS_TAC[binterl_rules]
-rewrite_tac[binterl_rules]
+rewrite_tac[binterl]
         
                 
-∀Sym P S1 S2 Sym' P' S1' S2' (MTrn1:('event1 + 'eventS, 'pred1, 'state1, 'symb) mtrel) (MTrn2:('event2 + 'eventS, 'pred2, 'state2, 'symb) mtrel) CMTrn CDed Ded1 Ded2 t. 
+∀t Sym P S1 S2 Sym' P' S1' S2' Ded1 Ded2. 
 ((FST ((MTrn1,Ded1) || (MTrn2,Ded2))) (Sym,P,S1,S2) t (Sym',P',S1',S2'))
-  ⇔
+⇔
     (∃t1 t2. (MTrn1 (Sym,(IMAGE OUTL P),S1) t1 (Sym',(IMAGE OUTL P'),S1')) ∧ (MTrn2 (Sym,(IMAGE OUTR P),S2) t2 (Sym',(IMAGE OUTR P'),S2')) ∧ (binterl t1 t2 t))
 
-
+CCONTR_TAC
 REPEAT GEN_TAC>>
     EQ_TAC>>
     rewrite_tac[composeMultiOperation_def]>>
@@ -91,16 +123,21 @@ REPEAT GEN_TAC>>
     Induct_on `t1`
     Induct_on `t2`
 rewrite_tac[binterl_nil]
-FULL_SIMP_TAC (list_ss++pred_setSimps.PRED_SET_ss++boolSimps.LIFT_COND_ss++boolSimps.EQUIV_EXTRACT_ss) [composeMuRe_def]
+FULL_SIMP_TAC (list_ss++pred_setSimps.PRED_SET_ss++boolSimps.LIFT_COND_ss++boolSimps.EQUIV_EXTRACT_ss) [composeMuRe_nil]
 rw[]
 asm_rewrite_tac[]
 asm_rewrite_tac[]
-
+Cases_on `t2 = []`
+METIS_TAC[MTrn1_cases,MTrn1_rules,MTrn1_ind,MTrn1_nil,MTrn1_snoc]
+asm_rewrite_tac[MTrn1_cases,MTrn1_rules,MTrn1_ind,MTrn1_nil,MTrn1_snoc]
         gen_tac
 strip_tac
 Cases_on `h`
-Q.EXISTS_TAC `x::t1` >> Q.EXISTS_TAC `t2`
-        
+Cases_on `x`
+Cases_on `t1 = []`
+Q.EXISTS_TAC `[]` >> Q.EXISTS_TAC `[]`
+        Q.ID_SPEC_TAC `b`
+MP_TAC (Q.SPECL [`n1`, `NONE`, `(T, \_. T)`, `p`, `state0`] 
      Induct_on `t`
     Induct_on `t1`
     Induct_on `t2`
@@ -109,13 +146,13 @@ Q.EXISTS_TAC `x::t1` >> Q.EXISTS_TAC `t2`
         RES_TAC
     FULL_SIMP_TAC (list_ss++pred_setSimps.PRED_SET_ss++boolSimps.LIFT_COND_ss++boolSimps.EQUIV_EXTRACT_ss) [composeMuRe_def]
     FULL_SIMP_TAC (list_ss++pred_setSimps.PRED_SET_ss++boolSimps.LIFT_COND_ss++boolSimps.EQUIV_EXTRACT_ss) [BOTH_EXISTS_AND_THM]
-    METIS_TAC[binterl_rules]
+    METIS_TAC[composeMuRe_nil]
 rpt strip_tac
 rw[]
-
-
-
-
+MP_TAC (Q.SPECL [`t1`] binterl_rules)
+rename1 `[]`
+Q.EXISTS_TAC `[INL x']` >> Q.EXISTS_TAC `t2`
+PAT_X_ASSUM ``∀t1 t2. A`` (ASSUME_TAC o (Q.SPECL [`[]`,`[]`]))
         REPEAT GEN_TAC>>
     EQ_TAC>>
     rewrite_tac[composeMultiOperation_def]>>
@@ -123,9 +160,15 @@ rw[]
     Induct_on `t`>>
     strip_tac
      Q.EXISTS_TAC `[]` >> Q.EXISTS_TAC `[]`
-rewrite_tac[binterl_nil]
-FULL_SIMP_TAC (list_ss++pred_setSimps.PRED_SET_ss++boolSimps.LIFT_COND_ss++boolSimps.EQUIV_EXTRACT_ss) [composeMuRe_def]
+rewrite_tac[bin]
+FULL_SIMP_TAC (list_ss++pred_setSimps.PRED_SET_ss++boolSimps.LIFT_COND_ss++boolSimps.EQUIV_EXTRACT_ss) [MTrn1_nil]
 rw[]
+  PAT_X_ASSUM ``∃t1 t2.B`` (IMP_RES_TAC)
+ PAT_X_ASSUM ``A = BType_Imm Bit1`` (ASSUME_TAC)
+  IMP_RES_TAC AND_INTRO_THM
+  FULL_SIMP_TAC (list_ss++pred_setSimps.PRED_SET_ss++boolSimps.LIFT_COND_ss++boolSimps.EQUIV_EXTRACT_ss) [IMAGE_DEF,MAP,OUTR,OUTL,INL,INR]
+  rewrite_tac[AND_INTRO_THM]
+   FULL_SIMP_TAC (list_ss++pred_setSimps.PRED_SET_ss++boolSimps.LIFT_COND_ss++boolSimps.EQUIV_EXTRACT_ss) []
 *)
     
 val _ = export_theory();
