src/tools/parallelcomposition/parallelcompositionsimpleScript.sml
@@ -162,7 +162,52 @@ Define  `
  (∃Sym' P' S2' P1 P1' P2 P2'. (P = P1<+>P2)∧(P' = P1'<+>P2')∧(Re2 (Sym,P2,S2) [INL E] (Sym',P2',S2'))∧(P1 = P1')∧ (composeMuRe Re1 Re2 (Sym',P',S1,S2') ev (Sym'',P'',S1'',S2'')))) ∧
 ((composeMuRe (Re1:(('event1 + 'eventS), 'pred1, 'state1, 'symb) mtrel) (Re2:(('event2 + 'eventS), 'pred2, 'state2, 'symb) mtrel) (Sym,P,S1,S2) ((INR (INR (E:'eventS)))::ev) (Sym'',P'',S1'',S2'')) =
  (∃Sym1' Sym2' Sym' P' S1' S2' P1 P1' P2 P2'. (P = P1<+>P2)∧(P' = P1'<+>P2')∧(Re1 (Sym,P1,S1) [INR E] (Sym1',P1',S1'))∧(Re2 (Sym,P2,S2) [INR E] (Sym2',P2',S2'))∧(Sym' = Sym1'∪Sym2') ∧ (composeMuRe Re1 Re2 (Sym',P',S1',S2') ev (Sym'',P'',S1'',S2''))))
-`;      *)          
+`;      *)
+
+(*
+Inductive composeMuRe:
+[~nil:]
+  (composeMuRe (Re1:(('event1 + 'eventS), 'pred1, 'state1, 'symb) mtrel) (Re2:(('event2 + 'eventS), 'pred2, 'state2, 'symb) mtrel) (Sym,P,S1,S2) [] (Sym,P,S1,S2)) /\
+[~left:]
+  (((composeMuRe Re1 Re2 (Sym,P,S1,S2) ev (Sym',P',S1',S2')) /\ (Re1 (Sym',(IMAGE OUTL P'),S1') [INL e1] (Sym'',(IMAGE OUTL P''),S1'')) /\ ((IMAGE OUTR P') = (IMAGE OUTR P'')))
+                 ==> (composeMuRe Re1 Re2 (Sym,P,S1,S2) ((INL (INL e1))::ev) (Sym'',P'',S1'',S2'))) /\
+[~right:]                                                                        
+  (((composeMuRe Re1 Re2 (Sym,P,S1,S2) ev (Sym',P',S1',S2')) /\ (Re2 (Sym',(IMAGE OUTR P'),S2') [INL e2] (Sym'',(IMAGE OUTR P''),S2'')) /\ ((IMAGE OUTL P') = (IMAGE OUTL P'')))
+                 ==> (composeMuRe Re1 Re2 (Sym,P,S1,S2) ((INR (INL e2))::ev) (Sym'',P'',S1',S2''))) /\
+[~sync:]                                                                        
+  (((composeMuRe Re1 Re2 (Sym,P,S1,S2) ev (Sym',P',S1',S2')) /\ (Re1 (Sym',(IMAGE OUTL P'),S1') [INR es] (Sym1'',(IMAGE OUTL P''),S1'')) /\
+                 (Re2 (Sym',(IMAGE OUTR P'),S2') [INR es] (Sym2'',(IMAGE OUTR P''),S2'')) /\ (Sym''' = (Sym1'' ∪ Sym2'')))
+                 ==> (composeMuRe Re1 Re2 (Sym,P,S1,S2) ((INR (INR es))::ev) (Sym'',P'',S1',S2'')))
+End
+
+Definition composeMuRe:
+[~nil:]
+  (composeMuRe (Re1:(('event1 + 'eventS), 'pred1, 'state1, 'symb) mtrel) (Re2:(('event2 + 'eventS), 'pred2, 'state2, 'symb) mtrel) (Sym,P,S1,S2) [] (Sym,P,S1,S2)) /\
+[~left:]
+  (((composeMuRe Re1 Re2 (Sym,P,S1,S2) ev (Sym',P',S1',S2')) /\ (Re1 (Sym',(IMAGE OUTL P'),S1') [INL e1] (Sym'',(IMAGE OUTL P''),S1'')) /\ ((IMAGE OUTR P') = (IMAGE OUTR P'')))
+                 ==> (composeMuRe Re1 Re2 (Sym,P,S1,S2) ((INL (INL e1))::ev) (Sym'',P'',S1'',S2'))) /\
+[~right:]                                                                        
+  (((composeMuRe Re1 Re2 (Sym,P,S1,S2) ev (Sym',P',S1',S2')) /\ (Re2 (Sym',(IMAGE OUTR P'),S2') [INL e2] (Sym'',(IMAGE OUTR P''),S2'')) /\ ((IMAGE OUTL P') = (IMAGE OUTL P'')))
+                 ==> (composeMuRe Re1 Re2 (Sym,P,S1,S2) ((INR (INL e2))::ev) (Sym'',P'',S1',S2''))) /\
+[~sync:]                                                                        
+  (((composeMuRe Re1 Re2 (Sym,P,S1,S2) ev (Sym',P',S1',S2')) /\ (Re1 (Sym',(IMAGE OUTL P'),S1') [INR es] (Sym1'',(IMAGE OUTL P''),S1'')) /\
+                 (Re2 (Sym',(IMAGE OUTR P'),S2') [INR es] (Sym2'',(IMAGE OUTR P''),S2'')) /\ (Sym''' = (Sym1'' ∪ Sym2'')))
+                 ==> (composeMuRe Re1 Re2 (Sym,P,S1,S2) ((INR (INR es))::ev) (Sym'',P'',S1',S2'')))
+End   *)
+
+val composeMuRe_def =
+Define  `
+((composeMuRe (Re1:(('event1 + 'eventS), 'pred1, 'state1, 'symb) mtrel) (Re2:(('event2 + 'eventS), 'pred2, 'state2, 'symb) mtrel) (Sym,P,S1,S2) [] (Sym',P',S1',S2')) =
+         (((Sym,P,S1,S2) = (Sym',P',S1',S2'))∧(Re1 (Sym,(IMAGE OUTL P),S1) [] (Sym,(IMAGE OUTL P),S1))∧(Re2 (Sym,(IMAGE OUTR P),S2) [] (Sym,(IMAGE OUTR P),S2))))  ∧
+((composeMuRe (Re1:(('event1 + 'eventS), 'pred1, 'state1, 'symb) mtrel) (Re2:(('event2 + 'eventS), 'pred2, 'state2, 'symb) mtrel) (Sym,P,S1,S2) ((INL (INL (E:'event1)))::ev) (Sym'',P'',S1'',S2')) =
+ (∃Sym' P' S1'. (Re1 (Sym',(IMAGE OUTL P'),S1') [INL E] (Sym'',(IMAGE OUTL P''),S1''))∧((IMAGE OUTR P') = (IMAGE OUTR P''))∧ (composeMuRe Re1 Re2 (Sym,P,S1,S2) ev (Sym',P',S1',S2')))) ∧
+((composeMuRe (Re1:(('event1 + 'eventS), 'pred1, 'state1, 'symb) mtrel) (Re2:(('event2 + 'eventS), 'pred2, 'state2, 'symb) mtrel) (Sym,P,S1,S2) ((INR (INL (E:'event2)))::ev) (Sym'',P'',S1',S2'')) =
+ (∃Sym' P' S2'. (Re2 (Sym',(IMAGE OUTR P'),S2') [INL E] (Sym'',(IMAGE OUTR P''),S2''))∧((IMAGE OUTL P') = (IMAGE OUTL P''))∧ (composeMuRe Re1 Re2 (Sym,P,S1,S2) ev (Sym',P',S1',S2')))) ∧
+((composeMuRe (Re1:(('event1 + 'eventS), 'pred1, 'state1, 'symb) mtrel) (Re2:(('event2 + 'eventS), 'pred2, 'state2, 'symb) mtrel) (Sym,P,S1,S2) ((INR (INR (E:'eventS)))::ev) (Sym'',P'',S1'',S2'')) =
+ (∃Sym1'' Sym2'' Sym' P' S1' S2'. (Re1 (Sym',(IMAGE OUTL P'),S1') [INR E] (Sym1'',(IMAGE OUTL P''),S1''))∧(Re2 (Sym',(IMAGE OUTR P'),S2') [INR E] (Sym2'',(IMAGE OUTR P''),S2''))∧(Sym'' = Sym1''∪Sym2'') ∧ (composeMuRe Re1 Re2 (Sym,P,S1,S2) ev (Sym',P',S1',S2'))))
+`;
+      
+(*
 val composeMuRe_def =
 Define  `
         ((composeMuRe (Re1:(('event1 + 'eventS), 'pred1, 'state1, 'symb) mtrel) (Re2:(('event2 + 'eventS), 'pred2, 'state2, 'symb) mtrel) (Sym,P,S1,S2) [] (Sym',P',S1',S2')) =
@@ -173,7 +218,7 @@ Define  `
  (∃Sym' P' S2'. (Re2 (Sym,(IMAGE OUTR P),S2) [INL E] (Sym',(IMAGE OUTR P'),S2'))∧((IMAGE OUTL P) = (IMAGE OUTL P'))∧ (composeMuRe Re1 Re2 (Sym',P',S1,S2') ev (Sym'',P'',S1'',S2'')))) ∧
 ((composeMuRe (Re1:(('event1 + 'eventS), 'pred1, 'state1, 'symb) mtrel) (Re2:(('event2 + 'eventS), 'pred2, 'state2, 'symb) mtrel) (Sym,P,S1,S2) ((INR (INR (E:'eventS)))::ev) (Sym'',P'',S1'',S2'')) =
  (∃Sym1' Sym2' Sym' P' S1' S2'. (Re1 (Sym,(IMAGE OUTL P),S1) [INR E] (Sym1',(IMAGE OUTL P'),S1'))∧(Re2 (Sym,(IMAGE OUTR P),S2) [INR E] (Sym2',(IMAGE OUTR P'),S2'))∧(Sym' = Sym1'∪Sym2') ∧ (composeMuRe Re1 Re2 (Sym',P',S1',S2') ev (Sym'',P'',S1'',S2''))))
-`;
+`;*)
 
 (*
 val composeMuRe_def =
